vale/code/arch/x64/Vale.X64.State.fsti
@@ -40,9 +40,7 @@ unfold let eval_mem (ptr:int) (s:vale_state) : GTot nat64 = load_mem64 ptr s.vs_
 [@va_qattr]
 unfold let eval_mem128 (ptr:int) (s:vale_state) : GTot Vale.Def.Types_s.quad32 = load_mem128 ptr s.vs_heap
 [@va_qattr]
-unfold let eval_hpls (hp:nat) (s:vale_state) : vale_heap = Map.sel s.vs_memory.vm_hpls hp
-[@va_qattr]
-unfold let eval_hmap (ptr:int) (s:vale_state) : nat = Map.sel s.vs_memory.vm_hmap ptr
+unfold let eval_heap (hp:nat) (s:vale_state) : vale_heap = Map.sel s.vs_memory.vm_hpls hp
 [@va_qattr]
 unfold let eval_stack (ptr:int) (s:vale_state) : GTot nat64 = load_stack64 ptr s.vs_stack
 [@va_qattr]
@@ -95,15 +93,10 @@ let update_reg_xmm (r:reg_xmm) (v:quad32) (s:vale_state) : vale_state =
 let update_mem (ptr:int) (v:nat64) (s:vale_state) : GTot vale_state = {s with vs_heap = store_mem64 ptr v s.vs_heap}
 
 [@va_qattr]
-let update_hpls (hp:nat) (h:vale_heap) (s:vale_state) : vale_state = 
+let update_heap (hp:nat) (h:vale_heap) (s:vale_state) : vale_state = 
   let memory' = {s.vs_memory with vm_hpls = Map.upd s.vs_memory.vm_hpls hp h} in
   {s with vs_memory = memory'}
 
-[@va_qattr]
-let update_hmap (ptr:int) (hp:nat) (m: Map.t int nat) (s:vale_state) : vale_state =
-  let memory' = {s.vs_memory with vm_hmap = Map.upd s.vs_memory.vm_hmap ptr hp} in
-  {s with vs_memory = memory'}
-  
 [@va_qattr]
 let update_stack64 (ptr:int) (v:nat64) (s:vale_state) : GTot vale_state = {s with vs_stack = store_stack64 ptr v s.vs_stack}
 
